Fp/Theorems/Packing.lean
@@ -306,10 +306,10 @@ theorem toExtRat_eq_toExtRat' {pf : PackedFloat e s}
   cases hZero : pf.isZero <;>
   cases hNorm : pf.isNorm <;>
   all_goals simp only [toExtRat, toExtDyadic, ExtDyadic.toExtRat, toExtRat', hNaN, hInf, hZero, hNorm, cond_true,
-    cond_false, Dyadic.toRat_zero, PackedFloat.toNumberRat, PackedFloat.toNumberRatSig, PackedFloat.toNumberRatExp, Bool.false_eq_true, if_false, if_true]
+    cond_false, Dyadic.toRat_zero, PackedFloat.toNumberRat, PackedFloat.toRatSig, PackedFloat.toNumberRatExp, Bool.false_eq_true, if_false, if_true]
   all_goals simp only [Dyadic.toRat_ofIntWithPrec_eq_mul_two_pow, ExtRat.Number.injEq,
     Int.neg_add, Int.neg_sub, Bool.apply_cond]
-  -- all_goals (simp only [PackedFloat.toNumberRat, PackedFloat.toNumberRatSig, PackedFloat.toNumberRatExp, if_true, if_false, hNorm, Bool.false_eq_true])
+  -- all_goals (simp only [PackedFloat.toNumberRat, PackedFloat.toRatSig, PackedFloat.toNumberRatExp, if_true, if_false, hNorm, Bool.false_eq_true])
   all_goals (try simp only [BitVec.toInt_setWidth'_of_lt (Nat.lt_succ_self (s + 1)), Rat.intCast_natCast, BitVec.toInt_neg_eq_of_msb (BitVec.msb_setWidth'_of_lt (Nat.lt_succ_self (s + 1))), BitVec.toNat_cons', Bool.toNat, cond_false, cond_true, Nat.zero_shiftLeft, Nat.one_shiftLeft, Nat.zero_add, Int.natCast_add, Rat.intCast_neg, Rat.intCast_add, Rat.natCast_pow, Rat.natCast_ofNat])
   all_goals (cases pf.sign <;> simp only [cond_false, cond_true, Bool.toSign, if_true, Bool.false_eq_true, if_false, Rat.intCast_ofNat, Rat.intCast_neg, Rat.zero_add, Rat.one_mul, Rat.neg_mul])
   all_goals (rewrite [Rat.div_def])
@@ -386,7 +386,7 @@ theorem toExtRat_unpack_eq_toExtRat {pf : PackedFloat e s}
         · simp only [EUnpackedFloat.toExtRat, Bool.false_eq_true, ↓reduceIte, cond_false,
           EUnpackedFloat.isNaN_mkNumber, EUnpackedFloat.isInfinite_mkNumber,
           EUnpackedFloat.num_mkNumber, toExtRat', hNaN, hInf, ExtRat.Number.injEq]
-          simp only [PackedFloat.toNumberRat, PackedFloat.toNumberRatSig, PackedFloat.toNumberRatExp]
+          simp only [PackedFloat.toNumberRat, PackedFloat.toRatSig, PackedFloat.toNumberRatExp]
           simp [hNorm]
           rewrite [UnpackedFloat.toRat_normalize_eq_toRat UnpackedFloat.sigWidth_lt_exponentWidth_sub_one]
           · simp only [UnpackedFloat.toRat_eq, Rat.mul_assoc]
@@ -443,7 +443,7 @@ theorem toExtRat_unpack_eq_toExtRat {pf : PackedFloat e s}
           EUnpackedFloat.isNaN_mkNumber, EUnpackedFloat.isInfinite_mkNumber,
           EUnpackedFloat.num_mkNumber, toExtRat', hNaN, hInf,
           ExtRat.Number.injEq]
-          simp only [PackedFloat.toNumberRat, PackedFloat.toNumberRatSig, PackedFloat.toNumberRatExp, hNorm, if_true]
+          simp only [PackedFloat.toNumberRat, PackedFloat.toRatSig, PackedFloat.toNumberRatExp, hNorm, if_true]
           simp only [UnpackedFloat.toRat_eq, Rat.mul_assoc]
           congr 1
           simp only [BitVec.toNat_cons', Nat.shiftLeft_eq, Bool.toNat, cond_true]
